Superposition_Calculus: Removed not need assumption

thys/First_Order_Clause/Infinite_Variables_Per_Type.thy
@@ -3,25 +3,29 @@ theory Infinite_Variables_Per_Type
     "HOL-Library.Countable_Set"
     "HOL-Cardinals.Cardinals"
     Fresh_Identifiers.Fresh
+    Collect_Extra
 begin
 
 lemma infinite_prods:
-  fixes x :: "'a :: infinite"
+  assumes "infinite (UNIV :: 'a set)"
   shows "infinite {p :: 'a \<times> 'a. fst p = x}"
 proof -
   have "{p :: 'a \<times> 'a . fst p = x} = {x} \<times> UNIV"
     by auto
 
   then show ?thesis
-    using finite_cartesian_productD2 infinite_UNIV
+    using finite_cartesian_productD2 assms
     by auto
 qed
 
 lemma surj_infinite_set: "surj g \<Longrightarrow> infinite {x. f x = ty} \<Longrightarrow> infinite {x. f (g x) = ty}"
   by (smt (verit) UNIV_I finite_imageI image_iff mem_Collect_eq rev_finite_subset subset_eq)
 
-definition infinite_variables_per_type :: "('v \<Rightarrow> 'ty) \<Rightarrow> bool" where
-  "infinite_variables_per_type \<V> \<equiv> \<forall>ty. infinite {x. \<V> x = ty}"
+definition infinite_variables_per_type_on :: "'var set \<Rightarrow> ('var \<Rightarrow> 'ty) \<Rightarrow> bool" where
+  "infinite_variables_per_type_on X \<V> \<equiv> \<forall>ty \<in> \<V> ` X. infinite {x. \<V> x = ty}"
+
+abbreviation infinite_variables_per_type :: "('var \<Rightarrow> 'ty) \<Rightarrow> bool" where
+  "infinite_variables_per_type \<equiv> infinite_variables_per_type_on UNIV"
 
 lemma obtain_type_preserving_inj:
   fixes \<V> :: "'v \<Rightarrow> 'ty"
@@ -32,14 +36,15 @@ lemma obtain_type_preserving_inj:
     "inj f"
     "X \<inter> f ` Y = {}"
     "\<forall>x \<in> Y. \<V> (f x) = \<V> x"
-proof
+proof (rule that)
 
   {
     fix ty
+    assume "ty \<in> range \<V>"
 
-    have "|{x. \<V> x = ty}| =o |{x. \<V> x = ty } - X|"
+    then have "|{x. \<V> x = ty}| =o |{x. \<V> x = ty } - X|"
       using \<V> finite_X card_of_infinite_diff_finite ordIso_symmetric
-      unfolding infinite_variables_per_type_def
+      unfolding infinite_variables_per_type_on_def
       by blast
 
     then have "|{x. \<V> x = ty}| =o |{x. \<V> x = ty \<and> x \<notin> X}|"
@@ -66,12 +71,13 @@ proof
       by blast
 
     then have "f y \<in> {x. \<V> x = \<V> y \<and> x \<notin> X}"
-      using exists_g[of "\<V> y"]
-      unfolding f_def get_g_def
-      by (smt (verit, ccfv_threshold) someI)
+      using exists_g get_g_def
+      unfolding f_def 
+      by (metis (no_types, lifting) ext rangeI verit_sko_ex')     
   }
 
   then show "X \<inter> f ` Y = {}"  "\<forall>y\<in>Y. \<V> (f y) = \<V> y"
+    unfolding f_def
     by auto
 
   show "inj f"
@@ -82,7 +88,7 @@ proof
     then show "x = y"
       using get_g_def f_def exists_g
       unfolding some_eq_ex[symmetric]
-      by (smt (verit, ccfv_threshold) someI mem_Collect_eq bij_betw_iff_bijections)
+      by (smt (verit) bij_betw_iff_bijections mem_Collect_eq rangeI)
   qed
 qed
 
@@ -121,9 +127,108 @@ lemma obtain_type_preserving_injs':
   using obtain_type_preserving_injs[OF assms]
   by (metis inf_commute)
 
-lemma exists_infinite_variables_per_type:
+lemma obtain_infinite_variables_per_type_on:
+  assumes 
+    infinite_UNIV: "infinite (UNIV :: 'v set)" and 
+    finite_Y: "finite Y" and 
+    finite_Z: "finite Z" and 
+    disjoint: "Y \<inter> Z = {}"
+  obtains \<V> :: "'v \<Rightarrow> 'ty"
+  where "infinite_variables_per_type_on X \<V>" "\<forall>x \<in> Y. \<V> x = \<V>' x" "\<forall>x \<in> Z. \<V> x = \<V>'' x"
+proof (cases "X = {}")
+  case True
+  define \<V> where "\<And>x. \<V> x \<equiv> if x \<in> Y then \<V>' x else \<V>'' x"
+
+  show ?thesis
+  proof (rule that[unfolded True])
+
+    show "\<forall>x\<in>Y. \<V> x = \<V>' x"
+      unfolding \<V>_def
+      by simp
+  next
+
+    show "\<forall>x\<in>Z. \<V> x = \<V>'' x"
+      using disjoint
+      unfolding \<V>_def
+      by auto
+  qed (auto simp: infinite_variables_per_type_on_def)
+next
+  case False
+
+  obtain g :: "'v \<Rightarrow> 'v \<times> 'v" where bij_g: "bij g"
+    using Times_same_infinite_bij_betw_types bij_betw_inv infinite_UNIV 
+    by blast
+
+  define f :: "'v \<Rightarrow> 'v" where
+    "\<And>x. f x \<equiv> if x \<in> Y \<union> Z then x else fst (g x)"
+
+  define \<V> where "\<And>x. \<V> x \<equiv> if x \<in> Y then \<V>' x else \<V>'' x"
+
+  {
+    fix y
+
+    have "{x. fst (g x) = y} = inv g ` {p. fst p = y}"
+      by (smt (verit, ccfv_SIG) Collect_cong bij_g bij_image_Collect_eq bij_imp_bij_inv inv_inv_eq)
+
+    then have "infinite {x. fst (g x) = y}"
+      using infinite_prods[OF infinite_UNIV]
+      by (metis bij_g bij_is_surj finite_imageI image_f_inv_f)
+
+    then have "infinite {x. x \<notin> Y \<union> Z \<and> fst (g x) = y}"
+      using finite_Y finite_Z
+      unfolding Collect_not_mem_conj_eq
+      by simp
+
+    then have "infinite {x. f x = y}"
+      unfolding f_def if_distrib if_distribR Collect_if_eq 
+      by blast
+  }
+
+  then have \<V>_X: "\<forall>y \<in> \<V> ` f ` X. infinite {x. \<V> (f x) = y}"
+    by (smt (verit, best) Collect_mono imageE rev_finite_subset)
+
+  show ?thesis
+  proof (rule that)
+    show "infinite_variables_per_type_on X (\<V> \<circ> f)"
+      using \<V>_X
+      unfolding infinite_variables_per_type_on_def comp_def
+      by (metis image_image)
+  next
+    show "\<forall>x\<in>Y. (\<V> \<circ> f) x = \<V>' x"
+      unfolding f_def \<V>_def
+      by auto
+  next
+    show "\<forall>x\<in>Z. (\<V> \<circ> f) x = \<V>'' x"
+      using disjoint
+      unfolding f_def \<V>_def
+      by auto
+  qed
+qed
+
+lemma obtain_infinite_variables_per_type_on':
+  assumes infinite_UNIV: "infinite (UNIV :: 'v set)" and finite_Y: "finite Y" 
+  obtains \<V> :: "'v \<Rightarrow> 'ty"
+  where "infinite_variables_per_type_on X \<V>" "\<forall>x \<in> Y. \<V> x = \<V>' x"
+  using obtain_infinite_variables_per_type_on[OF infinite_UNIV finite_Y, of "{}"]
+  by auto
+
+lemma obtain_infinite_variables_per_type_on'':
+  assumes "finite Y"
+  obtains \<V> :: "'v :: infinite \<Rightarrow> 'ty"
+  where "infinite_variables_per_type_on X \<V>" "\<forall>x \<in> Y. \<V> x = \<V>' x"
+  using obtain_infinite_variables_per_type_on'[OF infinite_UNIV assms].
+
+lemma infinite_variables_per_type_on_subset: 
+  "X \<subseteq> Y \<Longrightarrow> infinite_variables_per_type_on Y \<V> \<Longrightarrow> infinite_variables_per_type_on X \<V>"
+  unfolding infinite_variables_per_type_on_def
+  by blast
+
+definition infinite_variables_for_all_types :: "('v \<Rightarrow> 'ty) \<Rightarrow> bool" where
+  "infinite_variables_for_all_types \<V> \<equiv> \<forall>ty. infinite {x. \<V> x = ty}"
+
+lemma exists_infinite_variables_for_all_types:
   assumes "|UNIV :: 'ty set| \<le>o |UNIV :: ('v :: infinite) set|"
-  shows "\<exists>\<V> :: 'v \<Rightarrow> 'ty. infinite_variables_per_type \<V>"
+  shows "\<exists>\<V> :: 'v \<Rightarrow> 'ty. infinite_variables_for_all_types \<V>"
 proof-
   obtain g :: "'v \<Rightarrow> 'v \<times> 'v" where bij_g: "bij g"
     using Times_same_infinite_bij_betw_types bij_betw_inv infinite_UNIV
@@ -140,7 +245,7 @@ proof-
 
     then have "infinite {x. f x = y}"
       unfolding f_def
-      using infinite_prods
+      using infinite_prods[OF infinite_UNIV]
       by (metis bij_g bij_is_surj finite_imageI image_f_inv_f)
   }
 
@@ -152,14 +257,19 @@ proof-
     by (smt (verit, ccfv_SIG) Collect_mono finite_subset surjD)
 
   then show ?thesis
-    unfolding infinite_variables_per_type_def
+    unfolding infinite_variables_for_all_types_def
     by meson
 qed
 
-lemma obtain_infinite_variables_per_type:
+lemma obtain_infinite_variables_for_all_types:
   assumes "|UNIV :: 'ty set| \<le>o |UNIV :: 'v set|"
-  obtains \<V> :: "'v :: infinite \<Rightarrow> 'ty" where "infinite_variables_per_type \<V>"
-  using exists_infinite_variables_per_type[OF assms]
+  obtains \<V> :: "'v :: infinite \<Rightarrow> 'ty" where "infinite_variables_for_all_types \<V>"
+  using exists_infinite_variables_for_all_types[OF assms]
+  by blast
+
+lemma infinite_variables_per_type_if_infinite_variables_for_all_types:
+  "infinite_variables_for_all_types \<V> \<Longrightarrow> infinite_variables_per_type \<V>"
+  unfolding infinite_variables_for_all_types_def infinite_variables_per_type_on_def
   by blast
 
 end
